proof-libs/fstar/core/Alloc.Collections.Vec_deque.fsti
@@ -1,0 +1,24 @@
+module Alloc.Collections.Vec_deque
+open Rust_primitives
+
+type t_VecDeque: Type0 -> unit -> Type0
+
+val impl_5__push_back #t #a (v: t_VecDeque t a) (x: t): t_VecDeque t a
+
+val impl_5__len #t #a (v: t_VecDeque t a): usize
+
+val impl_5__pop_front #t #a (v: t_VecDeque t a): t_VecDeque t a & Core.Option.t_Option t
+
+
+[@FStar.Tactics.Typeclasses.tcinstance]
+val from_vec_deque_array t a n: Core.Convert.t_From (Alloc.Collections.Vec_deque.t_VecDeque t a)
+        (Rust_primitives.Arrays.t_Array t
+            (Rust_primitives.Integers.mk_usize n))
+
+[@FStar.Tactics.Typeclasses.tcinstance]
+val index_vec_deque t a: Core.Ops.Index.t_Index (Alloc.Collections.Vec_deque.t_VecDeque t a)
+        Rust_primitives.Integers.usize
+
+[@FStar.Tactics.Typeclasses.tcinstance]
+val update_at t a: Rust_primitives.Hax.update_at_tc (Alloc.Collections.Vec_deque.t_VecDeque t a)
+        Rust_primitives.Integers.usize
