proof-libs/fstar/core/Alloc.Slice.fsti
@@ -7,3 +7,5 @@ let impl__to_vec #a (s: t_Slice a): t_Vec a Alloc.Alloc.t_Global = s
 let impl__into_vec #t #a (s: Alloc.Boxed.t_Box (t_Slice t) a): t_Vec t a = s
 
 val impl__concat #t1 #t2 (s: t_Slice t1): t_Slice t2
+
+val impl__sort_by #t (s: t_Slice t) (f: t -> t -> Core.Cmp.t_Ordering): t_Slice t
