proof-libs/fstar/core/Alloc.Vec.Drain.fsti
@@ -1,0 +1,6 @@
+module Alloc.Vec.Drain
+
+val t_Drain: Type0 -> unit -> Type0
+
+[@FStar.Tactics.Typeclasses.tcinstance]
+val iterator_drain t a: Core.Iter.Traits.Iterator.iterator (t_Drain t a)
